ROOT
@@ -2,9 +2,9 @@ chapter AFP
 
 session Diagonal (AFP) = Undirected_Graph_Theory +
   options [timeout = 300]
-  sessions "HOL-Library"
+  sessions "HOL-Library" "Stirling_Formula"
   theories
-    Diagonal
+    Far_From_Diagonal
   document_files
     "root.tex"
     "root.bib"
